@base <https://github.com/aantakli/aantakli.github.io/edit/main/vocabularies/actn-ns/index.html> .
@prefix : <https://github.com/aantakli/aantakli.github.io/edit/main/vocabularies/actn-ns/index.html> .
@prefix actn: <http://www.ajan-agents.de/vocabularies/actn-ns/#> .
@prefix ajan: <http://www.ajan-agents.de/vocabularies/ajan-ns/#> .
@prefix bt: <http://www.ajan-agents.de/vocabularies/behavior/bt-ns/#> .
@prefix owl: <http://www.w3.org/2002/07/owl#> .
@prefix rdf: <http://www.w3.org/1999/02/22-rdf-syntax-ns#> .
@prefix xml: <http://www.w3.org/XML/1998/namespace> .
@prefix xsd: <http://www.w3.org/2001/XMLSchema#> .
@prefix rdfs: <http://www.w3.org/2000/01/rdf-schema#> .
@prefix http: <http://www.w3.org/2006/http#> .
@prefix http-hdr: <http://www.w3.org/2008/http-headers#> .
@prefix http-mth: <http://www.w3.org/2008/http-methods#> .

# ---------------------------------------------------
# Action Classes
# ---------------------------------------------------

actn:Action 
	rdf:type rdfs:Class ,
			 owl:Class ;
	rdfs:comment "A AJAN Action" ;
	rdfs:isDefinedBy : ,
		<https://github.com/aantakli/AJAN-service/wiki/AJAN-Actions> ;
    rdfs:label "Action" .

actn:Communication 
	rdf:type rdfs:Class ,
			 owl:Class ;
	rdfs:comment "Specifies whether an action responds directly with the action result or asynchronously" ;
	rdfs:isDefinedBy : ,
		<https://github.com/aantakli/AJAN-service/wiki/AJAN-Actions> ;
    rdfs:label "Communication" .

actn:ServiceAction 
	rdf:type rdfs:Class ,
			 owl:Class ;
	rdfs:comment "A AJAN Action which is executed in the agent LD-domain" ;
	rdfs:isDefinedBy : ,
		<https://github.com/aantakli/AJAN-service/wiki/AJAN-Actions> ;
    rdfs:label "ServiceAction" ;
	rdfs:subClassOf actn:Action .

actn:PluginAction 
	rdf:type rdfs:Class ,
			 owl:Class ;
	rdfs:comment "A AJAN Action which is executed internally via a AJAN Plugin" ;
	rdfs:isDefinedBy : ,
		<https://github.com/aantakli/AJAN-service/wiki/AJAN-Actions> ;
    rdfs:label "PluginAction" ;
	rdfs:subClassOf actn:Action .

actn:Synchronous 
	rdf:type rdfs:Class ,
			 owl:Class ;
	rdfs:comment "An Action which response directly with its result" ;
	rdfs:isDefinedBy : ,
		<https://github.com/aantakli/AJAN-service/wiki/AJAN-Actions> ;
    rdfs:label "Synchronous" ;
	rdfs:subClassOf actn:Communication .

actn:Asynchronous 
	rdf:type rdfs:Class ,
			 owl:Class ;
	rdfs:comment "An Action which send its result asynchronously, the Action can therefore be aborted and has a RUNNING state" ;
	rdfs:isDefinedBy : ,
		<https://github.com/aantakli/AJAN-service/wiki/AJAN-Actions> ;
    rdfs:label "Asynchronous" ;
	rdfs:subClassOf actn:Communication .

actn:ActionVariable 
	rdf:type rdfs:Class ,
			 owl:Class ;
	rdfs:comment "A Variable in the form of ?VARIABLE which indicates the same resource used in Consumables and Producibles" ;
	rdfs:isDefinedBy : ,
		<https://github.com/aantakli/AJAN-service/wiki/AJAN-Actions> ;
    rdfs:label "ActionVariable" .

actn:Consumable 
	rdf:type rdfs:Class ,
			 owl:Class ;
	rdfs:comment "The preconditions of an Action or Goal represented as a SPARQL ASK query" ;
	rdfs:isDefinedBy : ,
		<https://github.com/aantakli/AJAN-service/wiki/AJAN-Actions> ;
    rdfs:label "Consumable" .

actn:Producible
	rdf:type rdfs:Class ,
			 owl:Class ;
	rdfs:comment "The postconditions of an Action or Goal represented as a SPARQL ASK query" ;
	rdfs:isDefinedBy : ,
		<https://github.com/aantakli/AJAN-service/wiki/AJAN-Actions> ;
    rdfs:label "Producible" .

actn:Binding
	rdf:type rdfs:Class ,
			 owl:Class ;
	rdfs:comment "Used in ServiceActions to define the HTTP binding to communicate with the action LD-resource in the agents domain" ;
	rdfs:isDefinedBy : ,
		<https://github.com/aantakli/AJAN-service/wiki/AJAN-Actions> ;
    rdfs:label "Producible" .

actn:Payload
	rdf:type rdfs:Class ,
			 owl:Class ;
	rdfs:comment "The binding payload for the HTTP request, defined as a SPARQL CONSTRUCT query" ;
	rdfs:isDefinedBy : ,
		<https://github.com/aantakli/AJAN-service/wiki/AJAN-Actions> ;
    rdfs:label "Producible" .



# ---------------------------------------------------
# Action Properties
# ---------------------------------------------------

actn:communication
	rdf:type rdf:Property ;
	rdfs:comment "Points to the communication type of that action" ;
    rdfs:label "communication" ;
	rdfs:isDefinedBy : ,
		<https://github.com/aantakli/AJAN-service/wiki/AJAN-Actions> ;
	rdfs:domain actn:Action ;
	rdfs:range actn:Communication .

actn:category
	rdf:type rdf:Property ;
	rdfs:comment "Points to a user specified category of that action" ;
    rdfs:label "category" ;
	rdfs:isDefinedBy : ,
		<https://github.com/aantakli/AJAN-service/wiki/AJAN-Actions> ;
	rdfs:domain actn:Action ;
	rdfs:range rdf:Resource .

actn:variables
	rdf:type rdf:Property ;
	rdfs:comment "Points to a rdf:List of ActionVariables" ;
    rdfs:label "variables" ;
	rdfs:isDefinedBy : ,
		<https://github.com/aantakli/AJAN-service/wiki/AJAN-Actions> ;
	rdfs:domain actn:Action ;
	rdfs:range rdf:List .

actn:consumes
	rdf:type rdf:Property ;
	rdfs:comment "Points to the Consumable of that action" ;
    rdfs:label "consumes" ;
	rdfs:isDefinedBy : ,
		<https://github.com/aantakli/AJAN-service/wiki/AJAN-Actions> ;
	rdfs:domain actn:Action ,
		ajan:Goal ;
	rdfs:range actn:Consumable .

actn:produces
	rdf:type rdf:Property ;
	rdfs:comment "Points to the Producible of that action" ;
    rdfs:label "produces" ;
	rdfs:isDefinedBy : ,
		<https://github.com/aantakli/AJAN-service/wiki/AJAN-Actions> ;
	rdfs:domain actn:Action ,
		ajan:Goal ;
	rdfs:range actn:Producible .

actn:runBinding
	rdf:type rdf:Property ;
	rdfs:comment "Points to the HTTP binding to run that action in the agent domain" ;
    rdfs:label "runBinding" ;
	rdfs:isDefinedBy : ,
		<https://github.com/aantakli/AJAN-service/wiki/AJAN-Actions> ;
	rdfs:domain actn:Action ;
	rdfs:range actn:Binding .

actn:abortBinding
	rdf:type rdf:Property ;
	rdfs:comment "Points to the HTTP binding to abort that action in the agent domain" ;
    rdfs:label "abortBinding" ;
	rdfs:isDefinedBy : ,
		<https://github.com/aantakli/AJAN-service/wiki/AJAN-Actions> ;
	rdfs:domain actn:Action ;
	rdfs:range actn:Binding .

actn:sparql 
	rdf:type rdf:Property ;
	rdfs:comment "Points the a SPARQL Query" ;
    rdfs:label "sparql " ;
	rdfs:isDefinedBy : ,
		<https://github.com/aantakli/AJAN-service/wiki/AJAN-Actions> ;
	rdfs:domain actn:Payload ,
		actn:Consumable ,
		actn:Producible ;
	rdfs:range xsd:string .

actn:varName
	rdf:type rdf:Property ;
	rdfs:comment "Points to the variable name of a Action Variable" ;
    rdfs:label "varName" ;
	rdfs:isDefinedBy : ,
		<https://github.com/aantakli/AJAN-service/wiki/AJAN-Actions> ;
	rdfs:domain actn:ActionVariable ;
	rdfs:range xsd:string .